checkpoint

monad/smonad2.v
@@ -3,117 +3,106 @@ Require Import Program.
 Section monad.
 Variable ST : Set.
 
-Definition ST_Pre : Type
+Definition CS_Pre : Type
   := ST -> Prop.
-(* xxx why bother with separate ST_Post? *)
-Definition ST_Post (A:Set) : Type :=
-  ST -> A -> ST -> Prop.
-Definition C_Post (A:Set) : Type :=
+Definition CS_Post (A:Set) : Type :=
   ST -> A -> nat -> ST -> Prop.
 
 Program Definition
-  CS (st_pre : ST_Pre) (A : Set) (st_post : ST_Post A)
-     (c_post : C_Post A) : Set :=
-  forall st : { st : ST | st_pre st },
-    { (a, st') : A * ST | st_post st a st' /\
-      (* xxx what if the proof requires knowing st_post? *)
-      exists an, c_post st a an st' }.
+  CS (pre : CS_Pre) (A : Set) (post : CS_Post A) : Set :=
+  forall st : { st : ST | pre st },
+    { (a, st') : A * ST | exists an, post st a an st' }.
 Hint Unfold CS.
 
-Definition top : ST_Pre := fun st => True.
+Definition top : CS_Pre := fun st => True.
 
-Program Definition ret (A : Set) (c_post : C_Post A) 
+Program Definition ret (A : Set) (post : CS_Post A) 
   : forall av,
-    (forall st, c_post st av 0 st) ->
-    CS top A (fun st ap st' => st = st' /\ ap = av) c_post.
+    (forall st, post st av 0 st) ->
+    CS top A (fun st ap an st' => st = st' /\ ap = av /\ post st ap an st').
 Proof.
-  intros A c_post av CPav0.
+  intros A post av CPav0.
   unfold CS.
-  intros [st st_pre_st].
+  intros [st pre_st].
   exists (av, st).
   eauto.
 Defined.
 
 Program Definition bind:
-  forall (A B:Set)
-    (st_preA : ST_Pre) (st_preB : A -> ST_Pre)
-    (st_postA : ST_Post A) (st_postB : A -> ST_Post B)
-    (c_postA : C_Post A) (c_postB : C_Post B),
-    (CS st_preA A st_postA c_postA) ->
-    (forall (a : A), (* xxx missing (pa:exists an, PA a an) from monad.v *)
-      (CS (st_preB a) B (st_postB a)
+  forall (A:Set)
+    (preA : CS_Pre) (postA : CS_Post A) (am:(CS preA A postA))
+    (B:Set) (preB : A -> CS_Pre) (postB : A -> CS_Post B)
+    (bf:(forall (a : A)
+      (posta:exists st0 an stA,
+        postA st0 a an stA),
+      (CS (preB a) B
         (fun stA b bn stB =>
           forall st0 an,
-            c_postA st0 a an stA ->
-            c_postB st0 b (an+bn) stB))) ->
+            postA st0 a an stA ->
+            postB a stA b (an+bn) stB)))),
     CS (fun st0 =>
-      st_preA st0 /\
-      (forall a stA,
-        st_postA st0 a stA ->
-        st_preB a stA))
+      preA st0 /\
+      (forall a an stA,
+        postA st0 a an stA ->
+        preB a stA))
     B
-    (fun st0 b stB =>
-      exists a, exists stA,
-        st_postA st0 a stA /\
-        st_postB a stA b stB)
-    c_postB.
+    (fun st0 b bn stB =>
+      exists a an stA,
+        postA st0 a an stA /\
+        postB a stA b bn stB).
 Proof.
-  intros. rename H into am. rename H0 into bf.
-  intros [st0 [st_preA_st0 st_postApreB]].
-  edestruct (am (exist st_preA st0 st_preA_st0))
-   as [[av stA] [st_postA_stA c_postA_stA]].
-  simpl in st_postA_stA.
-  assert (st_preB av stA) as st_preB_stA. eauto.
-  edestruct (bf av (exist (st_preB av) stA st_preB_stA)) as
-    [[bv stB] [st_postB_stB c_postApostB_stB]].
-  simpl in st_postB_stB.
+  intros.
+  intros [st0 [preA_st0 postApreB]].
+  edestruct (am (exist preA st0 preA_st0))
+   as [[av stA] postA_stA].
+  simpl in postA_stA.
+  assert (preB av stA) as preB_stA.
+  destruct postA_stA. eauto. simpl.
+  assert (exists (st0 : ST) (an : nat) (stA : ST), postA st0 av an stA) as postav.
+  destruct postA_stA. exists st0. exists x. exists stA. auto.
+  edestruct (bf av postav (exist (preB av) stA preB_stA)) as
+    [[bv stB] postApostB_stB].
+  simpl in postApostB_stB.
   exists (bv, stB).
-  split. exists av. exists stA. split.
-  simpl. auto. auto.
-
-  destruct c_postA_stA as [an c_postA_stA].
-  destruct c_postApostB_stB as [bn c_postApostB_stB].
-  exists (an + bn). eauto.
+  simpl.
+  destruct postA_stA as [an postA_stA].
+  destruct postApostB_stB as [bn postApostB_stB].
+  exists (an + bn). exists av. exists an. eauto. 
 Defined.
 
 Program Definition get:
-  CS top ST (fun st0 st1 st2 => st0 = st1 /\ st1 = st2)
-  (fun _ st1 st1n _ => st1n = 0).
+  CS top ST (fun st0 st1 gn st2 => st0 = st1 /\ gn = 0 /\ st2 = st0).
 Proof.
-  intros [st0 st_pre_st0].
+  intros [st0 pre_st0].
   exists (st0, st0). simpl.
   eauto.
 Defined.
 
 Program Definition put (st2:ST) :
-  CS top () (fun _ _ st2' => st2 = st2')
-  (fun _ _ un _ => un = 0).
+  CS top () (fun _ _ pn st2' => pn = 0 /\ st2 = st2').
 Proof.
-  intros st2 [st0 st_pre_st0].
+  intros st2 [st0 pre_st0].
   exists ((), st2).
   eauto.
 Defined.
 
 Program Definition inc (k:nat) :
-  forall (st_pre : ST_Pre) (A:Set) (st_post : ST_Post A) (c_post : C_Post A),
-    CS st_pre A st_post
+  forall (pre : CS_Pre) (A:Set) (post : CS_Post A),
+    CS pre A 
     (fun st a an st' =>
       forall am,
         an + k = am ->
-        c_post st a am st') ->
-    CS st_pre A st_post c_post.
+        post st a am st') ->
+    CS pre A post.
 Proof.
   intros. rename H into am.
-  intros [st0 st_pre_st0]. simpl.
-  edestruct (am (exist st_pre st0 st_pre_st0))
-   as [[av stA] [st_post_stA c_post_stA]].
+  intros [st0 pre_st0]. simpl.
+  edestruct (am (exist pre st0 pre_st0))
+   as [[av stA] post_stA].
   simpl in *.
   exists (av, stA).
-  split. auto.
-  destruct c_post_stA as [an c_post_stA].
-  exists (an + k).
-  eapply c_post_stA.
-  auto.
+  destruct post_stA as [an post_stA].
+  exists (an + k). eauto.
 Defined.
 
 End monad.
@@ -125,11 +114,6 @@ Section dumb_list.
   
 Definition ST := list nat.
 
-Definition ST_Pre_None : ST_Pre ST := (fun st => True).
-Hint Unfold ST_Pre_None.
-Definition ST_Post_Unchanged {A:Set} : ST_Post ST A := (fun st _ st' => st = st').
-Hint Unfold ST_Post_Unchanged.
-
 Program Fixpoint bare_list_insert x (l:list nat) : list nat :=
   match l with
     | nil =>
@@ -138,120 +122,524 @@ Program Fixpoint bare_list_insert x (l:list nat) : list nat :=
       (cons y (bare_list_insert x sl))
   end.
 
-(* XXX add that it equals bare_list_insert *)
 Program Fixpoint list_insert x (l:list nat) :
-  (@CS ST ST_Pre_None (list nat) ST_Post_Unchanged
-   (fun _ _ ln _ => ln = length l))
+  (@CS ST (fun st => True) (list nat)
+    (fun st r ln st' => r = bare_list_insert x l /\ ln = length l /\ st' = st))
   :=
   match l with
     | nil =>
-      (@ret ST (list nat) (fun _ _ ln _ => ln = length l) 
+      (@ret ST (list nat)
+        (fun st r ln st' => r = bare_list_insert x l /\ ln = length l /\ st' = st)
         (cons x nil) _)
     | cons y sl =>
-      (@bind ST (list nat) (list nat) ST_Pre_None (fun _ => ST_Pre_None)
-        ST_Post_Unchanged (fun _ => ST_Post_Unchanged)
-        (fun _ _ ln _ => ln = length sl)
-        (fun _ _ ln _ => ln = length l)
+      (@bind ST (list nat)
+        (fun st => True)
+        (fun st r ln st' => r = bare_list_insert x sl /\ ln = length sl /\ st' = st)
         (list_insert x sl)
-        (fun sl' =>
-          (@inc ST 1 ST_Pre_None (list nat) ST_Post_Unchanged
-            (fun _ _ ln _ => ln = length l)
-            (@ret ST (list nat) (fun _ _ ln _ => ln + 1 + length sl = length l)
+        (list nat)
+        (fun sl' st => sl' = bare_list_insert x sl)
+        (fun sl' st r ln st' => r = bare_list_insert x l /\ ln = length l /\ st' = st)
+        (fun sl' postsl' =>
+          (@inc ST 1 (fun st => True) (list nat)
+            (fun st r ln st' => r = bare_list_insert x l /\ ln = length l /\ st' = st)
+            (@ret ST (list nat)
+              (fun st r ln st' => r = bare_list_insert x l /\ ln = 0 /\ st' = st)
               (cons y sl') _))))
   end.
 
 Next Obligation.
-  simpl.
-  rename x0 into st.
-  rename H into Pre_st.
-  split. auto. eauto.
+  simpl. eauto.
 Defined.
 
 Next Obligation.
   simpl.
   rename x0 into st.
-  rename H into Pre_st.
-  split. auto.
+  rename H1 into Pre_st.
   exists (length sl). intros.
-  omega.
+  split. auto. split. omega. auto.
 Defined.
 
 Next Obligation.
   simpl.
   rename x0 into st.
-  rename H into Pre_st.
-  split. auto.
+  rename H4 into Pre_st.
   exists 1.
-  intros. omega.
+  intros st0 an [EQr [EQln EQst]].
+  split. auto. split. omega. auto.
+Defined.
+
+Next Obligation.
+  intuition.
 Defined.
 
 Next Obligation.
   simpl.
   rename x0 into st.
   rename H into ST_Pre_st.
-  destruct (list_insert x sl (exist ST_Pre_None st ST_Pre_st)) as [[sl' st'] IH].
-  destruct IH as [ST_Post_st' C_Post].
+  destruct (list_insert x sl (exist (fun _ : ST => True) st I)) as [[sl' st'] IH].
+  destruct IH as [sl'n [EQsl' [EQsl'n EQst]]].
   simpl in *.
-  split. auto.
-  destruct C_Post as [IHn C_Post].
-  exists (S IHn).
-  auto.
+  subst st' sl' sl'n.
+  eauto.
 Defined.
- 
+
 Program Definition insert (x:nat) :
   @CS ST
-  ST_Pre_None
+  (fun st => True)
   ()
-  (fun st _ st' => st' = bare_list_insert x st)
-  (fun st _ n _ => n = length st)
+  (fun st _ n st' => n = length st /\ st' = bare_list_insert x st)
   :=
-  @bind ST ST ()
-  ST_Pre_None
-  (fun st0v st0 => st0v = st0)
-  
-  (fun st0 st1 st2 => st0 = st1 /\ st1 = st2)
-  (fun st0v st0 _ st2 => st2 = bare_list_insert x st0)
-  
-  (fun st0 st0v getn st1 => getn = 0)
-  (fun st0 _ putn st2 => putn = length st0)
-  
+  @bind ST
+
+  ST
+  (fun st => True)
+  (fun st v vn st' => v = st /\ vn = 0 /\ st' = st)
   (@get ST)
-  (fun l =>
-    (@bind ST ST ()
+
+  ()
+  (fun av st => st = av)
+  (fun av st _ bn st' =>
+    st = av /\ bn = length st /\ st' = bare_list_insert x st)
+  (fun l postl =>
+    (@bind ST
+
+      ST 
       (fun st => st = l)
-      (fun _ st => st = l)
-      
-      ST_Post_Unchanged
-      (fun l' st _ st' => st' = l')
-      
-      (fun _ _ ln _ => ln = length l)
-      (fun st _ ln _ => ln = length st)
-      
+      (fun st l' l'n st' =>
+        l' = bare_list_insert x st /\ l'n = length st /\ st' = st)
       (list_insert x l)
-      (fun l' =>
+      
+      ()
+      (fun l' st => l' = bare_list_insert x st)
+      (fun l' st _ bn st' =>
+        l' = bare_list_insert x st /\ bn = length st /\ st' = l')
+      (fun l' postl' =>
         (@put ST l')))).
+
+Next Obligation.
+  simpl. eauto.
+Defined.
+
+Next Obligation.
+  destruct (list_insert x postl (exist (fun _ : ST => True) postl I))
+    as [[a st'] [an [EQa [EQan EQst']]]].
+  simpl in *.
+  eauto.
+Defined.
 
 Next Obligation.
   unfold top. auto.
 Defined.
 
 Next Obligation.
-  rename x0 into st0.
-  split. auto.
+  eexists. intros st0 an.
+  intros [EQr [EQan EQst]].
+  subst an x0. eauto.
+Defined.
 
-  (* XXX *)
-  exists (length st
+Next Obligation.
+  split; auto.
+  intros a an stA [EQa [EQan EQst]].
+  subst a an stA.
+  auto.
+Defined.
+
+(* XXX This "proof" is insane. What does it mean? *)
+Next Obligation.
+  program_simpl.
+  edestruct (list_insert x postl _).
+  
+  destruct (insert_obligation_6 x postl
+           (ex_intro
+              (fun st0 : ST =>
+               exists (an : nat) (stA : ST),
+                 postl = st0 /\ an = 0 /\ stA = st0) postl
+              (ex_intro
+                 (fun an : nat =>
+                  exists stA : ST, postl = postl /\ an = 0 /\ stA = postl) 0
+                 (ex_intro
+                    (fun stA : ST => postl = postl /\ 0 = 0 /\ stA = postl)
+                    postl (conj eq_refl (conj eq_refl eq_refl)))))
+           (exist (fun st : ST => st = postl) postl eq_refl)).
+  simpl in *.
+  remember (insert_obligation_3 x postl
+             (ex_intro
+                (fun st0 : ST =>
+                 exists (an : nat) (stA : ST),
+                   postl = st0 /\ an = 0 /\ stA = st0) postl
+                (ex_intro
+                   (fun an : nat =>
+                    exists stA : ST, postl = postl /\ an = 0 /\ stA = postl)
+                   0
+                   (ex_intro
+                      (fun stA : ST => postl = postl /\ 0 = 0 /\ stA = postl)
+                      postl (conj eq_refl (conj eq_refl eq_refl)))))
+             (exist (fun st : ST => st = postl) postl e)).
+  simpl in *.
+  clear Heqy.
+  destruct (list_insert x postl (exist (fun _ : ST => True) postl I)).
+  simpl in *.
+  destruct x0 as [a st]. simpl in *.
+  exists (length postl).
+  intros st0 an [EQp [EQan EQp2]].
+  subst.
+  repeat split; eauto.
+  destruct y. intuition.
+Qed.
+
+Next Obligation.
+  intuition. subst. auto.
+Qed.
+
+Next Obligation.
+  rename x0 into st0.
+  rename H into preA.
+  destruct (insert_obligation_8 x (exist (fun _ : ST => True) st0 preA))
+    as [preA_st0 postApreB].
+  simpl in *.
+  clear preA.
+  destruct (insert_obligation_1 x (exist (fun _ : ST => True) st0 preA_st0))
+    as [an postA_stA].
+  simpl in *.
+  clear preA_st0.
+  destruct postA_stA as [E0 [E1 E2]].
+  subst an.
+  
+  clear postApreB.
+  
+  
+  remember (insert_obligation_7 x x0
+             match
+               insert_obligation_1 x (exist (fun _ : ST => True) x0 preA_st0)
+             with
+             | ex_intro x1 H0 =>
+                 ex_intro
+                   (fun st0 : ST =>
+                    exists (an : nat) (stA : ST),
+                      x0 = st0 /\ an = 0 /\ stA = st0) x0
+                   (ex_intro
+                      (fun an : nat =>
+                       exists stA : ST, x0 = x0 /\ an = 0 /\ stA = x0) x1
+                      (ex_intro
+                         (fun stA : ST => x0 = x0 /\ x1 = 0 /\ stA = x0) x0
+                         H0))
+             end
+             (exist (fun st : ST => st = x0) x0
+                match
+                  insert_obligation_1 x
+                    (exist (fun _ : ST => True) x0 preA_st0)
+                with
+                | ex_intro x1 H0 => postApreB x0 x1 x0 H0
+                end)).
+  simpl in *.
+  rewrite <- Heqy.
+  clear Heqy.
+
+  
+  destruct ((let (bv, stB) as p
+             return
+               ((let (_, st') := p in
+                 exists an : nat,
+                   forall (st0 : ST) (an0 : nat),
+                   x0 = st0 /\ an0 = 0 /\ x0 = st0 ->
+                   x0 = x0 /\
+                   an0 + an = length x0 /\ st' = bare_list_insert x x0) ->
+                { (_, st') : () * ST |
+                exists (an : nat) (a0 : ST) (an0 : nat) 
+                (stA : ST),
+                  (a0 = x0 /\ an0 = 0 /\ stA = x0) /\
+                  stA = a0 /\ an = length stA /\ st' = bare_list_insert x stA}) :=
+             `
+             match
+               insert_obligation_6 x x0
+                 match
+                   insert_obligation_1 x
+                     (exist (fun _ : ST => True) x0 preA_st0)
+                 with
+                 | ex_intro x1 H0 =>
+                     ex_intro
+                       (fun st0 : ST =>
+                        exists (an : nat) (stA : ST),
+                          x0 = st0 /\ an = 0 /\ stA = st0) x0
+                       (ex_intro
+                          (fun an : nat =>
+                           exists stA : ST, x0 = x0 /\ an = 0 /\ stA = x0) x1
+                          (ex_intro
+                             (fun stA : ST => x0 = x0 /\ x1 = 0 /\ stA = x0)
+                             x0 H0))
+                 end
+                 (exist (fun st : ST => st = x0) x0
+                    match
+                      insert_obligation_1 x
+                        (exist (fun _ : ST => True) x0 preA_st0)
+                    with
+                    | ex_intro x1 H0 => postApreB x0 x1 x0 H0
+                    end)
+             with
+             | conj preA_st1 postApreB0 =>
+                 (let (av, stA) as p
+                      return
+                        ((let (a, st') := p in
+                          exists an : nat,
+                            a = bare_list_insert x x0 /\
+                            an = length x0 /\ st' = x0) ->
+                         { (_, st') : () * ST |
+                         exists (an : nat) (a0 : ST) 
+                         (an0 : nat) (stA : ST),
+                           (a0 = bare_list_insert x x0 /\
+                            an0 = length x0 /\ stA = x0) /\
+                           a0 = bare_list_insert x stA /\
+                           an = length stA /\ st' = a0}) :=
+                      `
+                      (list_insert x x0
+                         (exist (fun _ : ST => True) x0
+                            (insert_obligation_2 x x0
+                               match
+                                 insert_obligation_1 x
+                                   (exist (fun _ : ST => True) x0 preA_st0)
+                               with
+                               | ex_intro x1 H0 =>
+                                   ex_intro
+                                     (fun st0 : ST =>
+                                      exists (an : nat) 
+                                      (stA : ST),
+                                        x0 = st0 /\ an = 0 /\ stA = st0) x0
+                                     (ex_intro
+                                        (fun an : nat =>
+                                         exists stA : ST,
+                                           x0 = x0 /\ an = 0 /\ stA = x0) x1
+                                        (ex_intro
+                                           (fun stA : ST =>
+                                            x0 = x0 /\ x1 = 0 /\ stA = x0) x0
+                                           H0))
+                               end
+                               (exist (fun st : ST => st = x0) x0 preA_st1)))) in
+                  fun
+                    postA_stA : exists an : nat,
+                                  av = bare_list_insert x x0 /\
+                                  an = length x0 /\ stA = x0 =>
+                  exist
+                    (fun anonymous : () * ST =>
+                     let (_, st') := anonymous in
+                     exists (an : nat) (a0 : ST) (an0 : nat) 
+                     (stA0 : ST),
+                       (a0 = bare_list_insert x x0 /\
+                        an0 = length x0 /\ stA0 = x0) /\
+                       a0 = bare_list_insert x stA0 /\
+                       an = length stA0 /\ st' = a0) 
+                    ((), av)
+                    match postA_stA with
+                    | ex_intro an postA_stA0 =>
+                        match
+                          insert_obligation_5 x x0
+                            match
+                              insert_obligation_1 x
+                                (exist (fun _ : ST => True) x0 preA_st0)
+                            with
+                            | ex_intro x1 H0 =>
+                                ex_intro
+                                  (fun st0 : ST =>
+                                   exists (an0 : nat) 
+                                   (stA0 : ST),
+                                     x0 = st0 /\ an0 = 0 /\ stA0 = st0) x0
+                                  (ex_intro
+                                     (fun an0 : nat =>
+                                      exists stA0 : ST,
+                                        x0 = x0 /\ an0 = 0 /\ stA0 = x0) x1
+                                     (ex_intro
+                                        (fun stA0 : ST =>
+                                         x0 = x0 /\ x1 = 0 /\ stA0 = x0) x0
+                                        H0))
+                            end av
+                            match postA_stA with
+                            | ex_intro x1 H0 =>
+                                ex_intro
+                                  (fun st0 : ST =>
+                                   exists (an0 : nat) 
+                                   (stA0 : ST),
+                                     av = bare_list_insert x st0 /\
+                                     an0 = length st0 /\ stA0 = st0) x0
+                                  (ex_intro
+                                     (fun an0 : nat =>
+                                      exists stA0 : ST,
+                                        av = bare_list_insert x x0 /\
+                                        an0 = length x0 /\ stA0 = x0) x1
+                                     (ex_intro
+                                        (fun stA0 : ST =>
+                                         av = bare_list_insert x x0 /\
+                                         x1 = length x0 /\ stA0 = x0) stA H0))
+                            end
+                            (exist
+                               (fun st : ST => av = bare_list_insert x st)
+                               stA
+                               match postA_stA with
+                               | ex_intro x1 H0 => postApreB0 av x1 stA H0
+                               end)
+                        with
+                        | ex_intro bn postApostB_stB =>
+                            ex_intro
+                              (fun an0 : nat =>
+                               exists (a : ST) (an1 : nat) 
+                               (stA0 : ST),
+                                 (a = bare_list_insert x x0 /\
+                                  an1 = length x0 /\ stA0 = x0) /\
+                                 a = bare_list_insert x stA0 /\
+                                 an0 = length stA0 /\ av = a) 
+                              (an + bn)
+                              (ex_intro
+                                 (fun a : ST =>
+                                  exists (an0 : nat) 
+                                  (stA0 : ST),
+                                    (a = bare_list_insert x x0 /\
+                                     an0 = length x0 /\ stA0 = x0) /\
+                                    a = bare_list_insert x stA0 /\
+                                    an + bn = length stA0 /\ av = a) av
+                                 (ex_intro
+                                    (fun an0 : nat =>
+                                     exists stA0 : ST,
+                                       (av = bare_list_insert x x0 /\
+                                        an0 = length x0 /\ stA0 = x0) /\
+                                       av = bare_list_insert x stA0 /\
+                                       an + bn = length stA0 /\ av = av) an
+                                    (ex_intro
+                                       (fun stA0 : ST =>
+                                        (av = bare_list_insert x x0 /\
+                                         an = length x0 /\ stA0 = x0) /\
+                                        av = bare_list_insert x stA0 /\
+                                        an + bn = length stA0 /\ av = av) stA
+                                       (conj postA_stA0
+                                          (postApostB_stB x0 an postA_stA0)))))
+                        end
+                    end)
+                   (insert_obligation_3 x x0
+                      match
+                        insert_obligation_1 x
+                          (exist (fun _ : ST => True) x0 preA_st0)
+                      with
+                      | ex_intro x1 H0 =>
+                          ex_intro
+                            (fun st0 : ST =>
+                             exists (an : nat) (stA : ST),
+                               x0 = st0 /\ an = 0 /\ stA = st0) x0
+                            (ex_intro
+                               (fun an : nat =>
+                                exists stA : ST,
+                                  x0 = x0 /\ an = 0 /\ stA = x0) x1
+                               (ex_intro
+                                  (fun stA : ST =>
+                                   x0 = x0 /\ x1 = 0 /\ stA = x0) x0 H0))
+                      end (exist (fun st : ST => st = x0) x0 preA_st1))
+             end in
+         fun
+           postApostB_stB : exists an : nat,
+                              forall (st0 : ST) (an0 : nat),
+                              x0 = st0 /\ an0 = 0 /\ x0 = st0 ->
+                              x0 = x0 /\
+                              an0 + an = length x0 /\
+                              stB = bare_list_insert x x0 =>
+         exist
+           (fun anonymous : () * ST =>
+            let (_, st') := anonymous in
+            exists (an : nat) (a0 : ST) (an0 : nat) 
+            (stA : ST),
+              (a0 = x0 /\ an0 = 0 /\ stA = x0) /\
+              stA = a0 /\ an = length stA /\ st' = bare_list_insert x stA)
+           (bv, stB)
+           match
+             insert_obligation_1 x (exist (fun _ : ST => True) x0 preA_st0)
+           with
+           | ex_intro an postA_stA =>
+               match postApostB_stB with
+               | ex_intro bn postApostB_stB0 =>
+                   ex_intro
+                     (fun an0 : nat =>
+                      exists (a : ST) (an1 : nat) (stA : ST),
+                        (a = x0 /\ an1 = 0 /\ stA = x0) /\
+                        stA = a /\
+                        an0 = length stA /\ stB = bare_list_insert x stA)
+                     (an + bn)
+                     (ex_intro
+                        (fun a : ST =>
+                         exists (an0 : nat) (stA : ST),
+                           (a = x0 /\ an0 = 0 /\ stA = x0) /\
+                           stA = a /\
+                           an + bn = length stA /\
+                           stB = bare_list_insert x stA) x0
+                        (ex_intro
+                           (fun an0 : nat =>
+                            exists stA : ST,
+                              (x0 = x0 /\ an0 = 0 /\ stA = x0) /\
+                              stA = x0 /\
+                              an + bn = length stA /\
+                              stB = bare_list_insert x stA) an
+                           (ex_intro
+                              (fun stA : ST =>
+                               (x0 = x0 /\ an = 0 /\ stA = x0) /\
+                               stA = x0 /\
+                               an + bn = length stA /\
+                               stB = bare_list_insert x stA) x0
+                              (conj postA_stA
+                                 (postApostB_stB0 x0 an postA_stA)))))
+               end
+           end) y).
+  
+  destruct (insert_obligation_6 x x0
+              match
+                insert_obligation_1 x
+                  (exist (fun _ : ST => True) x0 preA_st0)
+              with
+              | ex_intro x1 H0 =>
+                  ex_intro
+                    (fun st0 : ST =>
+                     exists (an : nat) (stA : ST),
+                       x0 = st0 /\ an = 0 /\ stA = st0) x0
+                    (ex_intro
+                       (fun an : nat =>
+                        exists stA : ST, x0 = x0 /\ an = 0 /\ stA = x0) x1
+                       (ex_intro
+                          (fun stA : ST => x0 = x0 /\ x1 = 0 /\ stA = x0) x0
+                          H0))
+              end
+              (exist (fun st : ST => st = x0) x0
+                 match
+                   insert_obligation_1 x
+                     (exist (fun _ : ST => True) x0 preA_st0)
+                 with
+                 | ex_intro x1 H0 => postApreB x0 x1 x0 H0
+                 end))
+  as [preA_st1 postApreB0].
+  simpl in *.
+  
+  clear y.
+
+program_simpl.
+  
+  simpl in *.  
+  remember (insert_obligation_7 x x0
+             (ex_intro
+                (fun st0 : ST =>
+                 exists (an : nat) (stA : ST),
+                   x0 = st0 /\ an = 0 /\ stA = st0) x0
+                (ex_intro
+                   (fun an : nat =>
+                    exists stA : ST, x0 = x0 /\ an = 0 /\ stA = x0) x1
+                   (ex_intro (fun stA : ST => x0 = x0 /\ x1 = 0 /\ stA = x0)
+                      x0 a)))
+             (exist (fun st : ST => st = x0) x0 (e x0 x1 x0 a))).
+  simpl in *.
+  
   
   eauto.
   
-  destruct (`
-       (put ST (list_insert x st0)
-          (exist (fun st : ST => top ST st) st0
-             (insert_obligation_1 x st0
-                (exist (fun st : ST => st0 = st) st0 eq_refl))))) as [u st1].
+  exists (length postl).
+  destruct (list_insert x postl (exist (fun _ : ST => True) postl I))
+    as [[a st'] [an [EQa [EQan EQst']]]].
   
-  split.
- simpl.
+  eauto.
+  split. auto.
+  
+  eauto.
 
 End dumb_list.
 
+Recursive Extraction insert.
